Phi_Semantics_Framework/Phi_Semantics_Framework.thy
@@ -171,7 +171,7 @@ interpretation \<phi>empty_abnormal ABNM_CONS_OF by standard simp
 subsection \<open>All-in-One Semantics\<close>
 
 debt_axiomatization Well_Type :: \<open>TY \<Rightarrow> VAL set\<close>
-  where Well_Type_disjoint: \<open>ta \<noteq> tb \<Longrightarrow> Well_Type ta \<inter> Well_Type tb = {}\<close>
+(*  where Well_Type_disjoint: \<open>ta \<noteq> tb \<Longrightarrow> Well_Type ta \<inter> Well_Type tb = {}\<close> *)
 
 debt_axiomatization Can_EqCompare :: \<open>resource \<Rightarrow> VAL \<Rightarrow> VAL \<Rightarrow> bool\<close>
   where can_eqcmp_sym: "Can_EqCompare res A B \<longleftrightarrow> Can_EqCompare res B A"
@@ -184,11 +184,11 @@ consts EqCompare :: \<open>VAL \<Rightarrow> VAL \<Rightarrow> bool\<close>
 debt_axiomatization Zero :: \<open>TY \<Rightarrow> VAL option\<close>
   where zero_well_typ: "pred_option (\<lambda>v. v \<in> Well_Type T) (Zero T)"
 
-lemma Well_Type_unique:
+(* lemma Well_Type_unique:
   \<open>v \<in> Well_Type ta \<Longrightarrow> v \<in> Well_Type tb \<Longrightarrow> ta = tb\<close>
   using Well_Type_disjoint by blast
 
-abbreviation \<open>Valid_Type T \<equiv> Inhabited (Well_Type T)\<close>
+abbreviation \<open>Valid_Type T \<equiv> Inhabited (Well_Type T)\<close>*)
 
 
 subsection \<open>Fiction\<close>
